src/BuiltinSanity.v
@@ -1,0 +1,20 @@
+Require Import BuiltinSem.
+Require Import String.
+
+(* Sanity check to make sure all the prims are in the table above *)
+Lemma id_for_all_prims :
+  forall p,
+  exists s x y,
+    lookup s table = Some (mb x y p).
+Proof.
+  intros. 
+  unfold table.
+  destruct p;
+    unfold lookup;
+    do 3 eexists;
+  match goal with
+  | [ |- context[if string_dec ?X ?Y then _ else _] ] => instantiate (3 := X); simpl; reflexivity
+  end.
+  
+Qed.
+
