verif/BuiltinTestM.v
@@ -1,0 +1,15 @@
+Require Import Coqlib.
+Require Import EvalTac.
+Require Import Semantics.
+Require Import Values.
+Require Import AST.
+Require Import BuiltinTest.
+
+
+Lemma eval_mod :
+  eval_expr ge empty (EVar (246,"mod")) (bits (v 5)).
+Proof.
+  repeat e.
+  Unshelve.
+  all: exact nz.
+Qed.
