verif/BuiltinTestT.v
@@ -13,20 +13,3 @@ Proof.
   Unshelve.
   all: exact nz.
 Qed.
-
-
-Lemma eval_div :
-  eval_expr ge empty (EVar (245,"div")) (bits (v 5)).
-Proof.
-  repeat e.
-  Unshelve.
-  all: exact nz.
-Qed.
-
-Lemma eval_mod :
-  eval_expr ge empty (EVar (246,"mod")) (bits (v 5)).
-Proof.
-  repeat e.
-  Unshelve.
-  all: exact nz.
-Qed.
